Finish full functional specification for the RingBuffer

test/RingBuffer.fst
@@ -1,14 +1,30 @@
 module RingBuffer
 
+/// This module demonstrates how to implement a ringbuffer in Low*. It uses the
+/// new LowStar.Buffer abstraction, and demonstrates how to separate functional
+/// predicates from their low-level stateful counterparts.
+///
+/// TODO: add ``push_back`` and ``pop_back``
+
+/// We define the canonical abbreviations, taking care to shadow ST to make sure
+/// we don't end up referring to FStar.ST by accident.
 module B = LowStar.Buffer
 module U32 = FStar.UInt32
 module HS = FStar.HyperStack
 module M = LowStar.Modifies
 module ST = FStar.HyperStack.ST
+module S = FStar.Seq
 
+/// This brings into scope the ``!*`` and ``*=`` operators, which are
+/// specifically designed to operate on buffers of size 1, i.e. on pointers.
 open LowStar.BufferOps
 open FStar.HyperStack.ST
 
+/// A ringbuffer is a view over a buffer, with a start index, a length (i.e. how
+/// many elements are currently being stored) and a total length (i.e. the size
+/// of the underlying ``b``). We chose this style, as opposed to a pair of
+/// ``first`` and ``last`` indices, because it avoids modular arithmetic which
+/// would be difficult to reason about.
 noeq
 type t a = {
   b: B.buffer a;
@@ -17,36 +33,38 @@ type t a = {
   total_length: U32.t
 }
 
-// Some helpers...
+/// To facilitate writing predicates, we define a handy shortcut that is the
+/// reflection of the ``!*`` operator at the proof level.
 unfold
-let deref #a h (x: B.pointer a) = B.get h x 0
+let deref #a (h: HS.mem) (x: B.pointer a) = B.get h x 0
 
-let well_formed_f #a (h: HS.mem) (b: B.buffer a) (first length total_length: U32.t) =
+/// A first version of the well-formedness predicate for ring buffers. This
+/// predicate refers to a sequence, not a buffer, and therefore does not need
+/// the memory. It is useful in this module to have two versions of predicates:
+/// one that takes into account the memory, disjointness, etc. and another one
+/// that only focuses on index arithmetic. Nothing surprising here. Note that
+/// zero-sized ringbuffers are not allowed.
+let well_formed_f #a (b: S.seq a) (first length total_length: U32.t) =
   let open U32 in
-  B.length b = v total_length /\
+  S.length b = v total_length /\
   length <=^ total_length /\
   first <^ total_length /\
   total_length >^ 0ul
 
+/// Same predicate as above, but this time operating on a memory state and using
+/// a stateful ringbuffer.
 let well_formed #a (h: HS.mem) (x: t a) =
   B.live h x.b /\ B.live h x.first /\ B.live h x.length /\
   M.(loc_disjoint (loc_buffer x.b) (loc_buffer x.first)) /\
   M.(loc_disjoint (loc_buffer x.b) (loc_buffer x.length)) /\
   M.(loc_disjoint (loc_buffer x.first) (loc_buffer x.length)) /\
-  well_formed_f h x.b (deref h x.first) (deref h x.length) x.total_length
+  well_formed_f (B.as_seq h x.b) (deref h x.first) (deref h x.length) x.total_length
 
-// Avoiding the modulo operator at all costs; also: can't use !*x.first +
-// x.total_length -^ 1ul %^ x.total_length because this might overflow!
-let prev (i total_length: U32.t): Pure U32.t
-  (requires U32.(total_length >^ 0ul /\ i <^ total_length))
-  (ensures fun r -> U32.( r <^ total_length ))
-=
-  let open U32 in
-  if i >^ 0ul then
-    i -^ 1ul
-  else
-    total_length -^ 1ul
-
+/// We next define operators for moving around the ringbuffer with wraparound
+/// semantics. Defining this using a modulo operator is not a good idea, because:
+/// - writing ``i +^ 1ul %^ total_length`` may overflow
+/// - Z3 is notoriously bad at reasoning with modular arithmetic.
+/// So, instead, we just do a simple branch.
 let next (i total_length: U32.t): Pure U32.t
   (requires U32.(total_length >^ 0ul /\ i <^ total_length))
   (ensures fun r -> U32.( r <^ total_length ))
@@ -57,40 +75,111 @@ let next (i total_length: U32.t): Pure U32.t
   else
     i +^ 1ul
 
-let rec as_list_aux #a
-  (h: HS.mem)
-  (b: B.buffer a)
-  (first length total_length: U32.t): Ghost (list a)
-    (requires well_formed_f h b first length total_length)
-    (ensures fun _ -> True)
-    (decreases (U32.v length))
+let prev (i total_length: U32.t): Pure U32.t
+  (requires U32.(total_length >^ 0ul /\ i <^ total_length))
+  (ensures fun r -> U32.( r <^ total_length ))
 =
-  if U32.( length =^ 0ul ) then
-    []
+  let open U32 in
+  if i >^ 0ul then
+    i -^ 1ul
   else
-    B.get h b (U32.v first) ::
-      as_list_aux h b (next first total_length) U32.( length -^ 1ul ) total_length
+    total_length -^ 1ul
 
-let as_list #a (h: HS.mem) (x: t a): Ghost (list a)
-  (requires well_formed h x)
-  (ensures fun _ -> True)
-=
-  as_list_aux h x.b (deref h x.first) (deref h x.length) x.total_length
-
+/// These two are useful from the client's perspective, to capture how many slots
+/// are left in the buffer.
 let remaining_space #a (h: HS.mem) (x: t a { well_formed h x }) =
   U32.( x.total_length -^ (deref h x.length) )
 
 let space_left #a (h: HS.mem) (x: t a { well_formed h x }) =
   U32.( remaining_space h x >^ 0ul )
 
-let used_slot #a (h: HS.mem) (x: t a { well_formed h x }) (i: U32.t) =
-  let first = U32.v (deref h x.first) in
-  let length = U32.v (deref h x.length) in
-  let total_length = U32.v x.total_length in
+/// A predicate over indices that captures whether a given entry in the buffer
+/// is occupied. Once again, we avoid modular arithmetic by branching.
+let used_slot_f (first length total_length i: U32.t) =
+  let first = U32.v first in
+  let length = U32.v length in
+  let total_length = U32.v total_length in
   let i = U32.v i in
   first <= i /\ i < first + length \/
   first <= i + total_length /\ i + total_length < first + length
 
+/// Same thing, but over a memory and the actual references.
+let used_slot #a (h: HS.mem) (x: t a { well_formed h x }) (i: U32.t) =
+  let first = deref h x.first in
+  let length = deref h x.length in
+  let total_length = x.total_length in
+  used_slot_f first length total_length i
+
+/// We reflect a ringbuffer as a list. This is the functional version that
+/// operates over a sequence.
+let rec as_list_f #a
+  (b: S.seq a)
+  (first length total_length: U32.t): Ghost (list a)
+    (requires well_formed_f b first length total_length)
+    (ensures fun _ -> True)
+    (decreases (U32.v length))
+=
+  if U32.( length =^ 0ul ) then
+    []
+  else
+    S.index b (U32.v first) ::
+      as_list_f b (next first total_length) U32.( length -^ 1ul ) total_length
+
+/// The one central lemma of this module: assigning something in the unused
+/// parts of the buffer does not affect the contents of the list.
+let rec seq_update_unused_preserves_list (#a: eqtype)
+  (b: S.seq a)
+  (i: U32.t)
+  (e: a)
+  (first length total_length: U32.t): Lemma
+  (requires
+    U32.v i < S.length b /\
+    well_formed_f b first length total_length /\
+     ~(used_slot_f first length total_length i))
+  (ensures
+    well_formed_f b first length total_length /\ (
+    let b' = S.upd b (U32.v i) e in
+    as_list_f b first length total_length = as_list_f b' first length total_length
+  ))
+  (decreases (U32.v length))
+=
+  if U32.(length =^ 0ul) then
+    ()
+  else begin
+    seq_update_unused_preserves_list b i e (next first total_length)
+      U32.(length -^ 1ul) total_length
+  end
+
+/// This version is more convenient and refers to the current memory and buffer,
+/// as opposed to as sequence.
+let as_list #a (h: HS.mem) (x: t a): Ghost (list a)
+  (requires well_formed h x)
+  (ensures fun _ -> True)
+=
+  as_list_f (B.as_seq h x.b) (deref h x.first) (deref h x.length) x.total_length
+
+/// ``pop`` is easy to prove, and requires no particular call to a lemma,
+/// because we don't modify the underlying buffer. Since the buffer contents
+/// don't change, the total predicate ``as_list_f`` is preserved, and F* is able
+/// to prove automatically the functional specification.
+let pop (#a: eqtype) (x: t a): Stack a
+  (requires fun h ->
+    well_formed h x /\ U32.(deref h x.length >^ 0ul))
+  (ensures fun h0 r h1 ->
+    well_formed h1 x /\
+    M.(modifies (loc_union (loc_buffer x.length) (loc_buffer x.first)) h0 h1) /\
+    U32.(remaining_space h1 x = remaining_space h0 x +^ 1ul) /\ (
+    let hd :: tl = as_list h0 x in
+    r = hd /\ as_list h1 x = tl))
+=
+  let e = x.b.(!*x.first) in
+  let h0 = ST.get () in
+  x.first *= next !*x.first x.total_length;
+  x.length *= U32.(!*x.length -^ 1ul);
+  let h1 = ST.get () in
+  e
+
+/// ``push`` is slightly more involved and crucially relies on the lemma above.
 let push (#a: eqtype) (x: t a) (e: a): Stack unit
   (requires fun h ->
     well_formed h x /\ space_left h x)
@@ -100,28 +189,21 @@ let push (#a: eqtype) (x: t a) (e: a): Stack unit
     M.(modifies (loc_union
       (loc_buffer x.length)
         (loc_union (loc_buffer x.first) (loc_buffer x.b))) h0 h1) /\
-    True) // as_list h1 x = e :: as_list h0 x)
+    as_list h1 x = e :: as_list h0 x)
 =
   let dest_slot = prev !*x.first x.total_length in
+  let h0 = ST.get () in
   x.b.(dest_slot) <- e;
+  seq_update_unused_preserves_list (B.as_seq h0 x.b) dest_slot e
+    (deref h0 x.first) (deref h0 x.length) x.total_length;
   x.first *= dest_slot;
   x.length *= U32.(!*x.length +^ 1ul)
 
-let pop (#a: eqtype) (x: t a): Stack a
-  (requires fun h ->
-    well_formed h x /\ U32.(deref h x.length >^ 0ul))
-  (ensures fun h0 r h1 ->
-    well_formed h1 x /\
-    M.(modifies (loc_union (loc_buffer x.length) (loc_buffer x.first)) h0 h1) /\
-    U32.(remaining_space h1 x = remaining_space h0 x +^ 1ul) /\ (
-    let hd :: tl = as_list h0 x in
-    r = hd))// /\ as_list h1 x = tl))
-=
-  let e = x.b.(!*x.first) in
-  x.first *= next !*x.first x.total_length;
-  x.length *= U32.(!*x.length -^ 1ul);
-  e
-
+/// ``create`` leverages the ``StackInline`` effect, and allocates three buffers
+/// -- we encapsulate stack allocation in a separate function, which facilitates
+/// verification. Relying on KreMLin's support, ``create`` will be textually
+/// inlined at call-site so that the allocations are effectively in the caller's
+/// stack frame.
 let create (#a: eqtype) (init: a) (len: U32.t): StackInline (t a)
   (requires (fun _ -> U32.v len > 0))
   (ensures (fun h0 x h1 ->
@@ -130,6 +212,8 @@ let create (#a: eqtype) (init: a) (len: U32.t): StackInline (t a)
   let b = B.alloca init len in
   { b = b; first = B.alloca 0ul 1ul; length = B.alloca 0ul 1ul; total_length = len }
 
+/// This test is crafted for continuous integration, so that the return value is
+/// 0l, indicating success.
 let main (): St Int32.t =
   push_frame ();
   let rb = create 1l 32ul in
